proof/DynamicLemmas.thy
@@ -36,8 +36,8 @@ lemma find_firsts_min_in_subset: "f \<in># find_firsts s h v e \<Longrightarrow>
   using min_subset_min_finite
   by (metis set_mset_mono finite_set_mset)
 
-
-method elim_Ev = (elim EvFire.cases EvMatch.cases EvGather.cases EvSelect.cases EvConsume.cases EvGain.cases; clarsimp)
+(* Invert single-constructor relations *)
+method elim_Ev = (elim EvFire.cases EvMatch.cases EvGather.cases EvGain.cases; clarsimp)
 method intro_Ev = (intro EvMatches.intros EvMatch.intros EvGain.intros EvGather.intros EvSelect.intros EvConsume.intros)
 
 (* trivial *)
@@ -46,84 +46,113 @@ lemma EvFire_new_is_added:
    dnew \<subseteq># store'"
   by elim_Ev
 
+(*
 (* We only spend what we have - trivial *)
 lemma EvMatches_spent_is_subset:
   "rn | asub | store | h \<turnstile> matches \<Down> ahas | dspent | h' MATCHES \<Longrightarrow>
-  dspent \<subseteq># store"
+   store_of_used_facts dspent \<subseteq># store"
+  unfolding store_of_used_facts_def
 proof (induct rule: EvMatches.induct)
   case (EvMatchNil n a s h)
-  then show ?case by auto
+  then show ?case
+    by (auto simp add: used_facts_empty_def)
 next
-  case (EvMatchCons n a s h m ag fw s' h' ms ag' ds' h'')
+  case (EvMatchCons n a s h m ag ds h' ms ag' ds' h'')
   then show ?case
     apply elim_Ev
-    by (simp add: add.commute count_le_replicate_mset_subset_eq subset_mset.le_diff_conv2)+
+    apply (elim EvConsume.cases)
+     apply (simp add: used_facts_add_def used_facts_empty_def add.commute count_le_replicate_mset_subset_eq subset_mset.le_diff_conv2)
+(*    sledgehammer
+     apply (meson mset_subset_eq_exists_conv subset_mset.order_trans)
+    by (simp add: used_facts_add_def)
 qed
+*)
+    oops
+*)
 
 lemma EvFire_spent_is_subset:
   "asub | store \<turnstile> rul \<Down> dspent | dnew | store' FIRE \<Longrightarrow>
-   dspent \<subseteq># store"
-  apply (elim EvFire.cases; clarsimp)
-  using EvMatches_spent_is_subset
-  by simp
+   store_of_used_facts dspent \<subseteq># store"
+  by elim_Ev
+
+
 
 (* We only use what we spend *)
 lemma frame_constriction_EvMatches:
   "rn | asub | store  | h \<turnstile> matches \<Down> ahas | dspent | h' MATCHES \<Longrightarrow>
-   rn | asub | dspent | h \<turnstile> matches \<Down> ahas | dspent | h' MATCHES"
-proof (induct rule: EvMatches.induct)
+   store_of_used_facts dspent \<subseteq># ds' \<Longrightarrow> ds' \<subseteq># store \<Longrightarrow>
+   rn | asub | ds' | h \<turnstile> matches \<Down> ahas | dspent | h' MATCHES"
+unfolding store_of_used_facts_def
+proof (induct arbitrary: ds' rule: EvMatches.induct)
   case (EvMatchNil n a s h)
   then show ?case
     using EvMatches.intros by simp
 next
-  case (EvMatchCons n a s h m ag fw s' h' ms ag' ds' h'')
-  moreover have spent_smaller: "ds' \<subseteq># s'"
-    using EvMatchCons EvMatches_spent_is_subset by auto
-  ultimately show ?case
-    apply elim_Ev
-    apply (intro_Ev; (rule refl)?; simp)
-    using EvMatchCons.hyps
-     apply blast
-
-    apply (intro_Ev; (rule refl)?; simp)
-     apply (rule find_firsts_min_in_subset)
-       apply assumption
-      apply (metis add.commute count_le_replicate_mset_subset_eq filter_union_mset multiset_filter_mono subset_mset.le_diff_conv2)
-     apply (metis count_filter_mset count_greater_zero_iff count_replicate_mset find_firsts_in_store union_iff)
-    using EvMatchCons.hyps
-     apply blast
-    done
+  case (EvMatchCons n a s h m ag ds h' ms ag' ds' h'')
+  then show ?case
+    apply -
+    apply (unfold used_facts_add_def)
+    apply (elim EvFire.cases EvMatch.cases EvGather.cases EvGain.cases; clarsimp)
+    apply (elim EvConsume.cases EvSelect.cases; clarsimp)
+       apply (intro_Ev; (rule refl)?; (simp add: used_facts_add_def)?)
+        apply (metis count_inI count_le_replicate_mset_subset_eq le_zero_eq mset_subset_eq_add_left not_gr_zero subseteq_mset_def)
+       apply (metis (no_types, lifting) EvMatchCons.hyps(3) mset_subset_eq_add_right subset_mset.sup.absorb_iff1 subset_mset.sup.bounded_iff)
+      apply (intro_Ev; (rule refl)?; (simp add: used_facts_add_def)?)
+       apply (rule find_firsts_min_in_subset)
+         apply assumption
+    using multiset_filter_mono
+        apply blast
+       apply (smt count_inI count_le_replicate_mset_subset_eq find_firsts_in_store le_zero_eq mem_Collect_eq mset_subset_eq_add_left not_gr_zero set_mset_filter subset_mset.order.trans)
+    apply (metis (no_types, lifting) EvMatchCons.hyps(3) mset_subset_eq_add_right subset_mset.sup.absorb_iff1 subset_mset.sup.bounded_iff)
+      apply (intro_Ev; (rule refl)?; (simp add: used_facts_add_def)?)
+    apply (simp add: mset_subset_eqD)
+    using EvMatchCons.hyps(3) subset_mset.sup.boundedI
+    apply blast
+      apply (intro_Ev; (rule refl)?; (simp add: used_facts_add_def)?)
+       apply (rule find_firsts_min_in_subset)
+         apply assumption
+    using multiset_filter_mono
+        apply blast
+       apply (smt count_inI count_le_replicate_mset_subset_eq find_firsts_in_store le_zero_eq mem_Collect_eq mset_subset_eq_add_left not_gr_zero set_mset_filter subset_mset.order.trans)
+    using EvMatchCons.hyps(3) subset_mset.le_supI by blast
 qed
 
 lemma frame_constriction:
   "asub | store  \<turnstile> rul \<Down> dspent | dnew | store' FIRE \<Longrightarrow>
-   asub | dspent \<turnstile> rul \<Down> dspent | dnew | dnew   FIRE"
+   asub | store_of_used_facts dspent \<turnstile> rul \<Down> dspent | dnew | (dnew + (facts_retained dspent - facts_consumed dspent))   FIRE"
   apply elim_Ev
-  using frame_constriction_EvMatches EvFire.intros
-  by fastforce
+  using frame_constriction_EvMatches
+  apply (intro EvFire.intros; blast?)
+  apply (unfold store_of_used_facts_def)
+  by (metis add.commute multi_union_self_other_eq subset_mset.add_diff_inverse subset_mset.sup.cobounded1 sup_subset_mset_def)
 
 (* We only spend visible facts *)
 lemma spend_only_accessible_EvMatches:
   "rn | asub | store  | h \<turnstile> matches \<Down> ahas | dspent | h' MATCHES  \<Longrightarrow>
-   (\<forall>f \<in># dspent. can_see_fact asub f)"
+   (\<forall>f \<in># store_of_used_facts dspent. can_see_fact asub f)"
 proof (induct rule: EvMatches.induct)
   case (EvMatchNil n a s h)
-  then show ?case by simp
+  then show ?case
+    by (simp add: store_of_used_facts_def used_facts_add_def used_facts_empty_def)
 next
   case (EvMatchCons n a s h m ag fw s' h' ms ag' ds' h'')
   then show ?case
     apply elim_Ev
-    using check_gather_def
-     apply blast
-    using check_gather_def find_firsts_in_store
-    by (metis count_greater_zero_iff filter_mset.rep_eq neq0_conv)
+    apply (simp add: store_of_used_facts_def used_facts_add_def used_facts_empty_def)
+    apply (elim EvSelect.cases;
+           clarsimp)
+     apply (elim EvConsume.cases;
+            fastforce simp add: check_gather_def)
+    by (elim EvConsume.cases;
+        clarsimp;
+        smt UnCI check_gather_def find_firsts_in_store mem_Collect_eq set_mset_filter)
 qed
 
 lemma spend_only_accessible:
   "asub | store \<turnstile> rul \<Down> dspent | dnew | store' FIRE \<Longrightarrow>
-   (\<forall>f \<in># dspent. can_see_fact asub f)"
-  apply elim_Ev
-  using spend_only_accessible_EvMatches by blast
+   (\<forall>f \<in># store_of_used_facts dspent. can_see_fact asub f)"
+  by (elim EvFire.cases; force simp add: spend_only_accessible_EvMatches)
+
 
 lemma check_gather_inaccessible_empty:
   " (\<forall>f \<in># others. \<not>(can_see_fact asub f)) \<Longrightarrow>
@@ -144,66 +173,122 @@ next
   case (EvMatchCons n a s h m ag fw s' h' ms ag' ds' h'')
   then show ?case
     apply elim_Ev
-    apply (intro_Ev; (rule refl)?; simp?)
-     apply (metis (no_types, lifting) EvMatchCons.hyps(3) add.commute add.left_commute add_diff_cancel_left' count_le_replicate_mset_subset_eq subset_mset.add_diff_inverse)
-    apply (intro_Ev; (rule refl)?; simp?)
-     apply (subst check_gather_inaccessible_empty[where others=others]; simp)
-    by (metis EvMatchCons.hyps(3) count_le_replicate_mset_subset_eq subset_mset.add_diff_assoc2)
+    apply (elim EvSelect.cases)
+     apply (elim EvConsume.cases;
+            clarsimp)
+      apply (intro_Ev;
+            (rule refl)?;
+             simp?;
+             argo EvMatchCons.hyps)+
+    apply (intro_Ev;
+          (rule refl)?;
+          simp?)
+     apply (subst check_gather_inaccessible_empty[where others=others];
+            simp add: EvSelect.simps)
+    using EvMatchCons.hyps by blast
 qed
 
 lemma store_weaken_inaccessible:
   "asub |  store           \<turnstile> rul \<Down> dspent | dnew |  store'           FIRE \<Longrightarrow>
    (\<forall>f \<in># others. \<not>(can_see_fact asub f)) \<Longrightarrow>
    asub | (store + others) \<turnstile> rul \<Down> dspent | dnew | (store' + others) FIRE"
-  apply elim_Ev
+  apply (elim EvFire.cases; clarsimp)
   apply (intro EvFire.intros)
-  using store_weaken_inaccessible_EvMatches apply blast
-  apply blast
-  using EvMatches_spent_is_subset by fastforce
+  using store_weaken_inaccessible_EvMatches
+      apply blast
+     apply blast
+    apply (simp add: subset_mset.add_increasing2)
+   apply (metis ab_semigroup_add_class.add_ac(1) add.commute store_of_used_facts_def subset_mset.add_diff_assoc2 subset_mset.sup.bounded_iff)
+  by blast
 
 
 (* auth of new facts is subset of auth of all spent facts *)
 lemma new_auth_gained_from_spent_EvMatches:
   "rn | asub | store | h \<turnstile> matches \<Down> ahas | dspent | h' MATCHES  \<Longrightarrow>
-  \<forall>a \<in> ahas. \<exists>d \<in># dspent. a \<in> fact_by d"
-(* ahas \<subseteq> \<Union>(fact_by ` set_mset dspent) *)
+  \<forall>a \<in> ahas. \<exists>d \<in># store_of_used_facts dspent. a \<in> fact_by d"
 proof (induct rule: EvMatches.induct)
   case (EvMatchNil n a s h)
   then show ?case by simp
 next
   case (EvMatchCons n a s h m ag fw s' h' ms ag' ds' h'')
   then show ?case
-    by (elim_Ev; blast)
+    by (elim_Ev;
+        elim EvSelect.cases;
+        elim EvConsume.cases;
+        clarsimp simp add: store_of_used_facts_def used_facts_add_def used_facts_empty_def;
+        blast)
 qed
-
 
 lemma new_auth_gained_from_spent:
   "asub | store \<turnstile> rul \<Down> dspent | dnew | store' FIRE \<Longrightarrow>
-  \<forall>f \<in># dnew. \<forall>a \<in> fact_by f. \<exists>d \<in># dspent. a \<in> fact_by d"
-  apply elim_Ev
+  \<forall>f \<in># dnew. \<forall>a \<in> fact_by f. \<exists>d \<in># store_of_used_facts dspent. a \<in> fact_by d"
   using new_auth_gained_from_spent_EvMatches
-  by blast
+  by (elim EvFire.cases; blast)
 
 
-(* Question: what do we know about observer sets (fact_obs)? *)
+
+fun matches_only_any :: "match list \<Rightarrow> bool" where
+"matches_only_any matches = list_all (\<lambda>m. case m of match x gath sel con gain \<Rightarrow> sel = select_any) matches"
 
 fun rule_only_any :: "rule \<Rightarrow> bool" where
-"rule_only_any (rule _ matches _) = list_all (\<lambda>m. case m of match x gath sel con gain \<Rightarrow> sel = select_any) matches"
+"rule_only_any (rule _ matches _) = matches_only_any matches"
 
 (* More permissions never stops a program from running *)
 (* This probably isn't true for 'first' selectors, where adding more permissions could make a new minimum visible *)
 (* But if the program only contains any selectors, it is true *)
+lemma auth_weaken_EvMatches:
+  "rn |  asub           | store | h \<turnstile> matches \<Down> ahas | dspent | h' MATCHES  \<Longrightarrow>
+    matches_only_any matches \<Longrightarrow>
+   rn | (asub \<union> others) | store | h \<turnstile> matches \<Down> ahas | dspent | h' MATCHES"
+proof (induct rule: EvMatches.induct)
+case (EvMatchNil n a s h)
+  then show ?case
+    by (simp add: EvMatches.EvMatchNil)
+next
+  case (EvMatchCons n a s h m ag ds h' ms ag' ds' h'' ag'' ds'')
+  then show ?case
+    apply (elim_Ev)
+    apply (elim EvSelect.cases; clarsimp)
+     apply (intro_Ev; (rule refl)?; (simp add: check_gather_def can_see_fact_def)?)
+    using EvMatchCons.hyps(3) matches_only_any.elims
+    by blast+
+qed
+
 lemma auth_weaken:
   "asub           | store \<turnstile> rul \<Down> dspent | dnew | store' FIRE \<Longrightarrow>
     rule_only_any rul \<Longrightarrow>
   (asub \<union> others) | store \<turnstile> rul \<Down> dspent | dnew | store' FIRE"
-  oops
+  apply (elim EvFire.cases)
+  using auth_weaken_EvMatches
+  by (metis EvFire.intros diff_union_cancelL mset_subset_eq_exists_conv rule_only_any.simps union_commute)
+
 
 (* We can always add new facts if the program only contains 'any' selectors *)
+lemma store_weaken_if_any_EvMatches:
+  "rn | asub |  store            | h \<turnstile> matches \<Down> ahas | dspent | h' MATCHES  \<Longrightarrow>
+    matches_only_any matches \<Longrightarrow>
+   rn | asub | (store + others) | h \<turnstile> matches \<Down> ahas | dspent | h' MATCHES"
+proof (induct rule: EvMatches.induct)
+case (EvMatchNil n a s h)
+  then show ?case
+    by (simp add: EvMatches.EvMatchNil)
+next
+  case (EvMatchCons n a s h m ag ds h' ms ag' ds' h'' ag'' ds'')
+  then show ?case
+    apply (elim_Ev; elim EvSelect.cases; clarsimp)
+    apply (intro_Ev; (rule refl)?; simp?)
+    using EvMatchCons.hyps(3) matches_only_any.elims
+    by blast
+qed
+
 lemma store_weaken_if_any:
   "asub |  store            \<turnstile> rul \<Down> dspent | dnew | store' FIRE \<Longrightarrow>
    rule_only_any rul \<Longrightarrow>
-   asub | (store \<union># others) \<turnstile> rul \<Down> dspent | dnew | store' FIRE"
-  oops
+   asub | (store + others) \<turnstile> rul \<Down> dspent | dnew | (store' + others) FIRE"
+  apply (elim EvFire.cases EvExec.cases; clarsimp)
+  apply (intro EvFire.intros EvExec.intros; (rule refl)?; assumption?)
+    apply (simp add: store_weaken_if_any_EvMatches)
+   apply (simp add: subset_mset.add_increasing2)
+  by (metis add.commute add.left_commute store_of_used_facts_def subset_mset.add_diff_assoc subset_mset.dual_order.trans subset_mset.sup.cobounded1)
 
 end
